minuska/src/two_counters_driver.ml
@@ -1,0 +1,32 @@
+open ExampleLang
+
+let usage_msg = "two_counters_driver -m <number1> -n <number2> [-depth <number3> ]"
+
+let depth = ref 10
+
+let number1 = ref 10
+let number2 = ref 10
+
+
+let anon_fun mynum =
+  number := int_of_string mynum
+
+let speclist =
+  [
+    ("-depth", Arg.Set_int depth, "Maximal execution depth"),
+    ("-m", Arg.Set_int number1, "number1"),
+    ("-n", Arg.Set_int number2, "number2")
+  ]
+
+let () =
+  Arg.parse speclist anon_fun usage_msg;
+  (* Main functionality here *)
+  print_string "Hello world!\n";
+  print_string (string_of_int !number1);
+  print_string (string_of_int !number2);
+  print_string (string_of_int !depth);
+  let result = ExampleLang.Coq_two_counters.interp_loop_number !depth !number in
+  match result with
+  | None -> print_string "None"
+  | Some x -> print_string "Some"; print_string (string_of_int x)
+  
