minuska/theories/examples.v
@@ -1,7 +1,5 @@
 From Coq.Logic Require Import ProofIrrelevance.
 
-Require Extraction.
-Extraction Language OCaml.
 
 From Minuska Require Import
     prelude
@@ -11,11 +9,6 @@ From Minuska Require Import
     empty_builtin
     flattened
     naive_interpreter
-.
-
-Extract Inductive nat => "int"
-  [ "0" "(fun x -> x + 1)" ]
-  "(fun zero succ n -> if n=0 then zero () else succ (n-1))"
 .
 
 
@@ -236,6 +229,84 @@ Module example_1.
         my_number_inv g'
     .
 
-    Extraction "ExampleLang.ml" interp_loop_number.
-
 End example_1.
+
+
+Module two_counters.
+
+    Definition rule_1 : FlattenedRewritingRule :=
+        rule ("top" [< "state" [< ( "s" [< $"M" >]), $"N" >] >])
+          => ("top" [< "state" [< $"M", "s" [< $"N" >]  >] >])
+          requires []
+    .
+
+    (*Print rule_1.*)
+
+    Definition Γ : FlattenedRewritingTheory := [rule_1].
+
+    Definition interp :=
+        naive_interpreter Γ
+    .
+
+    Fixpoint interp_loop
+        (fuel : nat)
+        (g : GroundTerm)
+        : option GroundTerm
+    :=
+    match fuel with
+    | 0 => Some g
+    | S fuel' => g' ← interp g; interp_loop fuel' g'
+    end
+    .
+
+    Definition pair_to_state (mn : nat*nat) : GroundTerm :=
+        aoo_app _ _ (ao_app_ao (ao_operator "top")
+        (
+            ao_app_ao
+                (
+                ao_app_ao (ao_operator "state")
+                    (example_1.my_number' mn.1)
+                )
+                (example_1.my_number' mn.2)
+        )
+        )
+    .
+
+    Definition state_to_pair (g : GroundTerm) : option (nat*nat) :=
+    match g with
+    | aoo_app _ _ (ao_app_ao (ao_operator "top")
+        (ao_app_ao (ao_app_ao (ao_operator "state") (m')) n'))
+        => 
+            m ← example_1.my_number'_inv m';
+            n ← example_1.my_number'_inv n';
+            Some (m, n)
+    | _ => None
+    end
+    .
+
+    Lemma pair_state_inversion : forall m n,
+        state_to_pair (pair_to_state (m,n)) = Some (m,n)
+    .
+    Proof.
+        intros m n.
+        simpl.
+        rewrite bind_Some.
+        exists m.
+        split.
+        { rewrite example_1.my_number_inversion'. reflexivity. }
+        rewrite bind_Some.
+        exists n.
+        split.
+        { rewrite example_1.my_number_inversion'. reflexivity. }
+        reflexivity.
+    Qed.
+
+    Definition interp_loop_number fuel := 
+        fun m n =>
+        let og' := ((interp_loop fuel) ∘ pair_to_state) (m,n) in
+        g' ← og';
+        state_to_pair g'
+    .
+
+End two_counters.
+
