minuska/theories/extraction.v
@@ -1,0 +1,22 @@
+Require Extraction.
+Extraction Language OCaml.
+
+From Minuska Require Import examples.
+
+Extract Inductive nat => "int"
+  [ "0" "(fun x -> x + 1)" ]
+  "(fun zero succ n -> if n=0 then zero () else succ (n-1))"
+.
+
+
+
+Extraction
+    "ExampleLang.ml"
+    example_1.interp_loop_number
+.
+
+
+Extraction
+    "TwoCounters.ml"
+    example_1.interp_loop_number
+.
